@prefix : <http://bimerr.iot.linkeddata.es/def/material-properties#> .
@prefix owl: <http://www.w3.org/2002/07/owl#> .
@prefix rdf: <http://www.w3.org/1999/02/22-rdf-syntax-ns#> .
@prefix xml: <http://www.w3.org/XML/1998/namespace> .
@prefix xsd: <http://www.w3.org/2001/XMLSchema#> .
@prefix rdfs: <http://www.w3.org/2000/01/rdf-schema#> .
@base <http://bimerr.iot.linkeddata.es/def/material-properties#> .

<http://bimerr.iot.linkeddata.es/def/material-properties#> rdf:type owl:Ontology ;
                                                            <http://purl.org/dc/elements/1.1/creator> "María Poveda-Villalón (Ontology Engineering Group, Universidad Politécnica de Madrid)" ,
                                                                                                      "Serge Chávez-Feria (Ontology Engineering Group, Universidad Politécnica de Madrid)" ;
                                                            <http://purl.org/dc/elements/1.1/description> "The material properties ontology provides the vocabulary to describe the composition of building elements."@en ;
                                                            <http://purl.org/dc/elements/1.1/publisher> "http://www.oeg-upm.net/" ;
                                                            <http://purl.org/dc/elements/1.1/title> "Material properties ontology"@en ;
                                                            <http://purl.org/vocab/vann/preferredNamespacePrefix> "mat" ;
                                                            owl:versionInfo "0.0.8" .

#################################################################
#    Annotation properties
#################################################################

###  http://purl.org/dc/elements/1.1/creator
<http://purl.org/dc/elements/1.1/creator> rdf:type owl:AnnotationProperty .


###  http://purl.org/dc/elements/1.1/description
<http://purl.org/dc/elements/1.1/description> rdf:type owl:AnnotationProperty .


###  http://purl.org/dc/elements/1.1/license
<http://purl.org/dc/elements/1.1/license> rdf:type owl:AnnotationProperty .


###  http://purl.org/dc/elements/1.1/publisher
<http://purl.org/dc/elements/1.1/publisher> rdf:type owl:AnnotationProperty .


###  http://purl.org/dc/elements/1.1/title
<http://purl.org/dc/elements/1.1/title> rdf:type owl:AnnotationProperty .


###  http://purl.org/vocab/vann/preferredNamespacePrefix
<http://purl.org/vocab/vann/preferredNamespacePrefix> rdf:type owl:AnnotationProperty .


#################################################################
#    Object Properties
#################################################################

###  http://bimerr.iot.linkeddata.es/def/material-properties#hasMaterial
:hasMaterial rdf:type owl:ObjectProperty ;
             rdfs:comment "Relation between a construction component (Layer, profile, constituent) and the materials that define them."@en ;
             rdfs:label "has material"@en .


###  http://bimerr.iot.linkeddata.es/def/material-properties#hasMaterialConstituent
:hasMaterialConstituent rdf:type owl:ObjectProperty ;
                        rdfs:comment "A relation between a constituent set and the specific material constituents."@en ;
                        rdfs:label "has material constituent"@en .


###  http://bimerr.iot.linkeddata.es/def/material-properties#hasMaterialConstituentSet
:hasMaterialConstituentSet rdf:type owl:ObjectProperty ;
                           rdfs:comment "Relation between an element and its construction based in material constituents."@en ;
                           rdfs:label "has material constituent set"@en .


###  http://bimerr.iot.linkeddata.es/def/material-properties#hasMaterialLayer
:hasMaterialLayer rdf:type owl:ObjectProperty ;
                  rdfs:comment "A relation between a layer set and the specific material layers."@en ;
                  rdfs:label "has material layer"@en .


###  http://bimerr.iot.linkeddata.es/def/material-properties#hasMaterialLayerSet
:hasMaterialLayerSet rdf:type owl:ObjectProperty ;
                     rdfs:comment "Relation between an element and its construction based in material layers."@en ;
                     rdfs:label "has material layer set"@en .


###  http://bimerr.iot.linkeddata.es/def/material-properties#hasMaterialProfile
:hasMaterialProfile rdf:type owl:ObjectProperty ;
                    rdfs:comment "A relation between a profile set and the specific material profiles."@en ;
                    rdfs:label "has material profile"@en .


###  http://bimerr.iot.linkeddata.es/def/material-properties#hasMaterialProfileSet
:hasMaterialProfileSet rdf:type owl:ObjectProperty ;
                       rdfs:comment "Relation between an element and its construction based in material profiles."@en ;
                       rdfs:label "has material profile set"@en .


###  http://bimerr.iot.linkeddata.es/def/material-properties#hasProperty
:hasProperty rdf:type owl:ObjectProperty ;
             rdfs:comment "A relationship between a feature of interest and a property of that feature."@en ;
             rdfs:label "has property"@en .


###  http://bimerr.iot.linkeddata.es/def/material-properties#hasPropertySet
:hasPropertySet rdf:type owl:ObjectProperty ;
                rdfs:comment "Relationship to connect a material or building element to an specific set of properties."@en ;
                rdfs:label "has property set"@en .


###  http://bimerr.iot.linkeddata.es/def/material-properties#isMeasurementOfMaterial
:isMeasurementOfMaterial rdf:type owl:ObjectProperty ;
                         rdfs:comment "Relation between a measurement with a specific material."@en ;
                         rdfs:label "is measurement of material"@en .


###  https://saref.etsi.org/core/isMeasuredIn
<https://saref.etsi.org/core/isMeasuredIn> rdf:type owl:ObjectProperty ;
                                           rdfs:comment "A relationship identifying the unit of measure used for a certain entity."@en ;
                                           rdfs:label "is measured in"@en .


###  https://saref.etsi.org/core/relatesToMeasurement
<https://saref.etsi.org/core/relatesToMeasurement> rdf:type owl:ObjectProperty ;
                                                   rdfs:comment "A relationship between a property and the measurements it relates to."@en ;
                                                   rdfs:label "relates to measurement"@en .


###  https://saref.etsi.org/core/relatesToProperty
<https://saref.etsi.org/core/relatesToProperty> rdf:type owl:ObjectProperty ;
                                                rdfs:comment "A relationship between a measurement and the property it relates to."@en ;
                                                rdfs:label "relates to property"@en .


#################################################################
#    Data properties
#################################################################

###  http://bimerr.iot.linkeddata.es/def/material-properties#description
:description rdf:type owl:DatatypeProperty ;
             rdfs:range xsd:string ;
             rdfs:comment "Description of the entity."@en ;
             rdfs:label "description"@en .


###  http://bimerr.iot.linkeddata.es/def/material-properties#identifierInDatabase
:identifierInDatabase rdf:type owl:DatatypeProperty ;
                      rdfs:range xsd:string ;
                      rdfs:comment "A relationship to indicate the identifier used in the source database"@en ;
                      rdfs:label "identifier in database"@en .


###  http://bimerr.iot.linkeddata.es/def/material-properties#ifcIdentifier
:ifcIdentifier rdf:type owl:DatatypeProperty ;
               rdfs:range xsd:string ;
               rdfs:comment "Ifc identifier of the element in an IFC file."@en ;
               rdfs:label "ifc identifier"@en .


###  http://bimerr.iot.linkeddata.es/def/material-properties#name
:name rdf:type owl:DatatypeProperty ;
      rdfs:range xsd:string ;
      rdfs:comment "Name of the entity."@en ;
      rdfs:label "name"@en .


###  http://bimerr.iot.linkeddata.es/def/material-properties#position
:position rdf:type owl:DatatypeProperty ;
          rdfs:range xsd:integer ;
          rdfs:comment "Position of the layer."@en ;
          rdfs:label "position"@en .


###  http://bimerr.iot.linkeddata.es/def/material-properties#thickness
:thickness rdf:type owl:DatatypeProperty ;
           rdfs:range xsd:float ;
           rdfs:comment "Thickness of the layer."@en ;
           rdfs:label "thickness"@en .


###  http://bimerr.iot.linkeddata.es/def/material-properties#type
:type rdf:type owl:DatatypeProperty ;
      rdfs:range xsd:string ;
      rdfs:comment "Type of material layer."@en ;
      rdfs:label "type"@en .


###  https://saref.etsi.org/core/hasValue
<https://saref.etsi.org/core/hasValue> rdf:type owl:DatatypeProperty ;
                                       rdfs:comment "A relationship defining the value of a certain property, e.g., energy or power. Note that, even if numeric values are expected to enable reasoning, measurement values could use other datatypes."@en ;
                                       rdfs:label "has value"@en .


#################################################################
#    Classes
#################################################################

###  http://bimerr.iot.linkeddata.es/def/building#Element
<http://bimerr.iot.linkeddata.es/def/building#Element> rdf:type owl:Class ;
                                                       rdfs:subClassOf [ rdf:type owl:Restriction ;
                                                                         owl:onProperty :hasMaterial ;
                                                                         owl:allValuesFrom :Material
                                                                       ] ,
                                                                       [ rdf:type owl:Restriction ;
                                                                         owl:onProperty :hasMaterialConstituentSet ;
                                                                         owl:allValuesFrom :MaterialConstituentSet
                                                                       ] ,
                                                                       [ rdf:type owl:Restriction ;
                                                                         owl:onProperty :hasMaterialLayerSet ;
                                                                         owl:allValuesFrom :MaterialLayerSet
                                                                       ] ,
                                                                       [ rdf:type owl:Restriction ;
                                                                         owl:onProperty :hasMaterialProfileSet ;
                                                                         owl:allValuesFrom :MaterialProfileSet
                                                                       ] ,
                                                                       [ rdf:type owl:Restriction ;
                                                                         owl:onProperty :ifcIdentifier ;
                                                                         owl:cardinality "1"^^xsd:nonNegativeInteger
                                                                       ] ,
                                                                       [ rdf:type owl:Restriction ;
                                                                         owl:onProperty :name ;
                                                                         owl:cardinality "1"^^xsd:nonNegativeInteger
                                                                       ] ,
                                                                       [ rdf:type owl:Restriction ;
                                                                         owl:onProperty :description ;
                                                                         owl:maxCardinality "1"^^xsd:nonNegativeInteger
                                                                       ] ;
                                                       rdfs:comment "An element is a generalization of all components that make up an AEC product."@en ;
                                                       rdfs:label "Element"@en ;
                                                       rdfs:seeAlso "http://standards.buildingsmart.org/IFC/DEV/IFC4_1/OWL#IfcElement"@en .


###  http://bimerr.iot.linkeddata.es/def/material-properties#Material
:Material rdf:type owl:Class ;
          rdfs:subClassOf [ rdf:type owl:Restriction ;
                            owl:onProperty :hasPropertySet ;
                            owl:allValuesFrom :PropertySet
                          ] ,
                          [ rdf:type owl:Restriction ;
                            owl:onProperty :name ;
                            owl:allValuesFrom xsd:string
                          ] ,
                          [ rdf:type owl:Restriction ;
                            owl:onProperty :description ;
                            owl:maxCardinality "1"^^xsd:nonNegativeInteger
                          ] ,
                          [ rdf:type owl:Restriction ;
                            owl:onProperty :identifierInDatabase ;
                            owl:maxQualifiedCardinality "1"^^xsd:nonNegativeInteger ;
                            owl:onDataRange xsd:string
                          ] ;
          rdfs:comment "A homogeneous or inhomogeneous substance that can be used to form elements (physical products or their components). (Definition taken from IFC)"@en ;
          rdfs:label "Material"@en ;
          rdfs:seeAlso "http://standards.buildingsmart.org/IFC/DEV/IFC4_1/OWL#IfcMaterial" .


###  http://bimerr.iot.linkeddata.es/def/material-properties#MaterialConstituent
:MaterialConstituent rdf:type owl:Class ;
                     rdfs:subClassOf [ rdf:type owl:Restriction ;
                                       owl:onProperty :hasMaterial ;
                                       owl:allValuesFrom :Material
                                     ] ,
                                     [ rdf:type owl:Restriction ;
                                       owl:onProperty :name ;
                                       owl:allValuesFrom xsd:string
                                     ] ,
                                     [ rdf:type owl:Restriction ;
                                       owl:onProperty :description ;
                                       owl:maxCardinality "1"^^xsd:nonNegativeInteger
                                     ] ;
                     rdfs:comment "A single and identifiable part of an element which is constructed of a number of part (one or more) each having an individual material."@en ;
                     rdfs:label "Material constituent"@en ;
                     rdfs:seeAlso "http://standards.buildingsmart.org/IFC/DEV/IFC4_1/OWL#IfcMaterialConstituent"@en .


###  http://bimerr.iot.linkeddata.es/def/material-properties#MaterialConstituentSet
:MaterialConstituentSet rdf:type owl:Class ;
                        rdfs:subClassOf [ rdf:type owl:Restriction ;
                                          owl:onProperty :hasMaterialConstituent ;
                                          owl:minQualifiedCardinality "1"^^xsd:nonNegativeInteger ;
                                          owl:onClass :MaterialConstituent
                                        ] ,
                                        [ rdf:type owl:Restriction ;
                                          owl:onProperty :name ;
                                          owl:allValuesFrom xsd:string
                                        ] ,
                                        [ rdf:type owl:Restriction ;
                                          owl:onProperty :description ;
                                          owl:maxCardinality "1"^^xsd:nonNegativeInteger
                                        ] ;
                        rdfs:comment "A collection of individual material constituents, each assigning a material to a part of an element."@en ;
                        rdfs:label "Material constituent set"@en ;
                        rdfs:seeAlso "http://standards.buildingsmart.org/IFC/DEV/IFC4_1/OWL#IfcMaterialConstituentSet"@en .


###  http://bimerr.iot.linkeddata.es/def/material-properties#MaterialLayer
:MaterialLayer rdf:type owl:Class ;
               rdfs:subClassOf [ rdf:type owl:Restriction ;
                                 owl:onProperty :hasMaterial ;
                                 owl:allValuesFrom :Material
                               ] ,
                               [ rdf:type owl:Restriction ;
                                 owl:onProperty :name ;
                                 owl:allValuesFrom xsd:string
                               ] ,
                               [ rdf:type owl:Restriction ;
                                 owl:onProperty :position ;
                                 owl:cardinality "1"^^xsd:nonNegativeInteger
                               ] ,
                               [ rdf:type owl:Restriction ;
                                 owl:onProperty :description ;
                                 owl:maxCardinality "1"^^xsd:nonNegativeInteger
                               ] ,
                               [ rdf:type owl:Restriction ;
                                 owl:onProperty :thickness ;
                                 owl:maxCardinality "1"^^xsd:nonNegativeInteger
                               ] ;
               rdfs:comment "A single and identifiable part of an element which is constructed of a number of layers (one or more)."@en ;
               rdfs:label "Material layer"@en ;
               rdfs:seeAlso "http://standards.buildingsmart.org/IFC/DEV/IFC4_1/OWL#IfcMaterialLayer"@en .


###  http://bimerr.iot.linkeddata.es/def/material-properties#MaterialLayerSet
:MaterialLayerSet rdf:type owl:Class ;
                  rdfs:subClassOf [ rdf:type owl:Restriction ;
                                    owl:onProperty :hasMaterialLayer ;
                                    owl:minQualifiedCardinality "1"^^xsd:nonNegativeInteger ;
                                    owl:onClass :MaterialLayer
                                  ] ,
                                  [ rdf:type owl:Restriction ;
                                    owl:onProperty :name ;
                                    owl:allValuesFrom xsd:string
                                  ] ,
                                  [ rdf:type owl:Restriction ;
                                    owl:onProperty :description ;
                                    owl:maxCardinality "1"^^xsd:nonNegativeInteger
                                  ] ;
                  rdfs:comment "A designation by which materials of an element constructed of a number of material layers is known and through which the relative positioning of individual layers can be expressed."@en ;
                  rdfs:label "Material layer set"@en ;
                  rdfs:seeAlso "http://standards.buildingsmart.org/IFC/DEV/IFC4_1/OWL#IfcMaterialLayerSet"@en .


###  http://bimerr.iot.linkeddata.es/def/material-properties#MaterialProfile
:MaterialProfile rdf:type owl:Class ;
                 rdfs:subClassOf [ rdf:type owl:Restriction ;
                                   owl:onProperty :hasMaterial ;
                                   owl:allValuesFrom :Material
                                 ] ,
                                 [ rdf:type owl:Restriction ;
                                   owl:onProperty :name ;
                                   owl:allValuesFrom xsd:string
                                 ] ,
                                 [ rdf:type owl:Restriction ;
                                   owl:onProperty :description ;
                                   owl:maxCardinality "1"^^xsd:nonNegativeInteger
                                 ] ;
                 rdfs:comment "A single and identifiable cross section of an element which is constructed of a number of profiles (one or more)."@en ;
                 rdfs:label "Material profile"@en ;
                 rdfs:seeAlso "http://standards.buildingsmart.org/IFC/DEV/IFC4_1/OWL#IfcMaterialProfile"@en .


###  http://bimerr.iot.linkeddata.es/def/material-properties#MaterialProfileSet
:MaterialProfileSet rdf:type owl:Class ;
                    rdfs:subClassOf [ rdf:type owl:Restriction ;
                                      owl:onProperty :hasMaterialProfile ;
                                      owl:minQualifiedCardinality "1"^^xsd:nonNegativeInteger ;
                                      owl:onClass :MaterialProfile
                                    ] ,
                                    [ rdf:type owl:Restriction ;
                                      owl:onProperty :name ;
                                      owl:allValuesFrom xsd:string
                                    ] ,
                                    [ rdf:type owl:Restriction ;
                                      owl:onProperty :description ;
                                      owl:maxCardinality "1"^^xsd:nonNegativeInteger
                                    ] ;
                    rdfs:comment "A designation by which individual material(s) of a prismatic element (for example, beam or column) constructed of a single or multiple material profiles is known."@en ;
                    rdfs:label "Material profile set"@en ;
                    rdfs:seeAlso "http://standards.buildingsmart.org/IFC/DEV/IFC4_1/OWL#IfcMaterialProfileSet"@en .


###  http://bimerr.iot.linkeddata.es/def/material-properties#Measurement
:Measurement rdf:type owl:Class ;
             rdfs:subClassOf [ rdf:type owl:Restriction ;
                               owl:onProperty <https://saref.etsi.org/core/isMeasuredIn> ;
                               owl:allValuesFrom :UnitOfMeasure
                             ] ,
                             [ rdf:type owl:Restriction ;
                               owl:onProperty <https://saref.etsi.org/core/relatesToProperty> ;
                               owl:allValuesFrom :Property
                             ] ,
                             [ rdf:type owl:Restriction ;
                               owl:onProperty <https://saref.etsi.org/core/isMeasuredIn> ;
                               owl:qualifiedCardinality "1"^^xsd:nonNegativeInteger ;
                               owl:onClass :UnitOfMeasure
                             ] ,
                             [ rdf:type owl:Restriction ;
                               owl:onProperty <https://saref.etsi.org/core/relatesToProperty> ;
                               owl:qualifiedCardinality "1"^^xsd:nonNegativeInteger ;
                               owl:onClass :Property
                             ] ,
                             [ rdf:type owl:Restriction ;
                               owl:onProperty <https://saref.etsi.org/core/hasValue> ;
                               owl:cardinality "1"^^xsd:nonNegativeInteger
                             ] ;
             rdfs:comment "Measurements related to materials."@en ;
             rdfs:label "Measurement"@en .


###  http://bimerr.iot.linkeddata.es/def/material-properties#Property
:Property rdf:type owl:Class ;
          rdfs:subClassOf [ rdf:type owl:Restriction ;
                            owl:onProperty <https://saref.etsi.org/core/relatesToMeasurement> ;
                            owl:allValuesFrom :Measurement
                          ] ,
                          [ rdf:type owl:Restriction ;
                            owl:onProperty :name ;
                            owl:cardinality "1"^^xsd:nonNegativeInteger
                          ] ,
                          [ rdf:type owl:Restriction ;
                            owl:onProperty :description ;
                            owl:maxCardinality "1"^^xsd:nonNegativeInteger
                          ] ;
          rdfs:comment "Properties of materials."@en ;
          rdfs:label "Property"@en .


###  http://bimerr.iot.linkeddata.es/def/material-properties#PropertySet
:PropertySet rdf:type owl:Class ;
             rdfs:subClassOf [ rdf:type owl:Restriction ;
                               owl:onProperty :hasProperty ;
                               owl:allValuesFrom :Property
                             ] ,
                             [ rdf:type owl:Restriction ;
                               owl:onProperty :hasProperty ;
                               owl:minCardinality "1"^^xsd:nonNegativeInteger
                             ] ,
                             [ rdf:type owl:Restriction ;
                               owl:onProperty :ifcIdentifier ;
                               owl:allValuesFrom xsd:string
                             ] ,
                             [ rdf:type owl:Restriction ;
                               owl:onProperty :name ;
                               owl:allValuesFrom xsd:string
                             ] ,
                             [ rdf:type owl:Restriction ;
                               owl:onProperty :description ;
                               owl:maxCardinality "1"^^xsd:nonNegativeInteger
                             ] ;
             rdfs:comment "N-ary class to unite specific properties related to building elements or materials."@en ;
             rdfs:label "Property set"@en .


###  http://bimerr.iot.linkeddata.es/def/material-properties#UnitOfMeasure
:UnitOfMeasure rdf:type owl:Class ;
               rdfs:subClassOf [ rdf:type owl:Restriction ;
                                 owl:onProperty :name ;
                                 owl:cardinality "1"^^xsd:nonNegativeInteger
                               ] ;
               rdfs:comment "The unit of measure is a standard for measurement of a quantity, such as a Property. For example, Power is a property and Watt is a unit of power that represents a definite predetermined power: when we say 10 Watt, we actually mean 10 times the definite predetermined power called watt. Our definition is based on the definition of unit of measure in the Ontology of units of Measure (OM). We propose here a list of some units of measure that are relevant for the purpose of SAREF, but this list can be extended, also using some other ontologies rather than the Ontology of units of Measure (OM)."@en ;
               rdfs:label "Unit of Measure"@en .


###  Generated by the OWL API (version 5.1.14) https://github.com/owlcs/owlapi/
